examples/riscv/chacha/chacha_symb_exec_quarterroundScript.sml
@@ -14,78 +14,9 @@ val _ = new_theory "chacha_symb_exec_quarterround";
 
 val _ = show_tags := true;
 
-(* ------------ *)
-(* quarterround *)
-(* ------------ *)
-
-(*
-   108a0:	00ab0a3b          	addw	s4,s6,a0
-   108a4:	014d4d33          	xor	s10,s10,s4
-   108a8:	010d151b          	slliw	a0,s10,0x10
-   108ac:	010d5d1b          	srliw	s10,s10,0x10
-   108b0:	01a56533          	or	a0,a0,s10
-
-   108b4:	01c5043b          	addw	s0,a0,t3
-   108b8:	008b4b33          	xor	s6,s6,s0
-   108bc:	00cb179b          	slliw	a5,s6,0xc
-   108c0:	014b5b1b          	srliw	s6,s6,0x14
-   108c4:	0167e7b3          	or	a5,a5,s6
-*)
-
-(*
-        <|bb_label :=
-            BL_Address_HC (Imm64 0x108A0w) "00AB0A3B (addw s4,s6,a0)";
-          bb_statements :=
-            [BStmt_Assign (BVar "x20" (BType_Imm Bit64))
-               (BExp_Cast BIExp_SignedCast
-                  (BExp_Cast BIExp_LowCast
-                     (BExp_BinExp BIExp_Plus
-                        (BExp_Den (BVar "x10" (BType_Imm Bit64)))
-                        (BExp_Den (BVar "x22" (BType_Imm Bit64)))) Bit32)
-                  Bit64)];
-          bb_last_statement :=
-            BStmt_Jmp (BLE_Label (BL_Address (Imm64 0x108A4w)))|>;
-        <|bb_label :=
-            BL_Address_HC (Imm64 0x108A4w) "014D4D33 (xor s10,s10,s4)";
-          bb_statements :=
-            [BStmt_Assign (BVar "x26" (BType_Imm Bit64))
-               (BExp_BinExp BIExp_Xor
-                  (BExp_Den (BVar "x20" (BType_Imm Bit64)))
-                  (BExp_Den (BVar "x26" (BType_Imm Bit64))))];
-          bb_last_statement :=
-            BStmt_Jmp (BLE_Label (BL_Address (Imm64 0x108A8w)))|>;
-        <|bb_label :=
-            BL_Address_HC (Imm64 0x108A8w) "010D151B (slliw a0,s10,0x10)";
-          bb_statements :=
-            [BStmt_Assign (BVar "x10" (BType_Imm Bit64))
-               (BExp_Cast BIExp_SignedCast
-                  (BExp_BinExp BIExp_LeftShift
-                     (BExp_Cast BIExp_LowCast
-                        (BExp_Den (BVar "x26" (BType_Imm Bit64))) Bit32)
-                     (BExp_Const (Imm32 16w))) Bit64)];
-          bb_last_statement :=
-            BStmt_Jmp (BLE_Label (BL_Address (Imm64 0x108ACw)))|>;
-        <|bb_label :=
-            BL_Address_HC (Imm64 0x108ACw) "010D5D1B (srliw s10,s10,0x10)";
-          bb_statements :=
-            [BStmt_Assign (BVar "x26" (BType_Imm Bit64))
-               (BExp_Cast BIExp_SignedCast
-                  (BExp_BinExp BIExp_RightShift
-                     (BExp_Cast BIExp_LowCast
-                        (BExp_Den (BVar "x26" (BType_Imm Bit64))) Bit32)
-                     (BExp_Const (Imm32 16w))) Bit64)];
-          bb_last_statement :=
-            BStmt_Jmp (BLE_Label (BL_Address (Imm64 0x108B0w)))|>;
-        <|bb_label :=
-            BL_Address_HC (Imm64 0x108B0w) "01A56533 (or a0,a0,s10)";
-          bb_statements :=
-            [BStmt_Assign (BVar "x10" (BType_Imm Bit64))
-               (BExp_BinExp BIExp_Or
-                  (BExp_Den (BVar "x10" (BType_Imm Bit64)))
-                  (BExp_Den (BVar "x26" (BType_Imm Bit64))))];
-          bb_last_statement :=
-            BStmt_Jmp (BLE_Label (BL_Address (Imm64 0x108B4w)))|>;
-*)
+(* ---------- *)
+(* first line *)
+(* ---------- *)
 
 val symb_analysis_thm =
  bir_symb_analysis_thm
@@ -97,6 +28,10 @@ val _ = Portable.pprint Tag.pp_tag (tag symb_analysis_thm);
 
 Theorem chacha_line_symb_analysis_thm = symb_analysis_thm
 
+(* ----------- *)
+(* second line *)
+(* ----------- *)
+
 val symb_analysis_thm =
  bir_symb_analysis_thm
   bir_chacha_prog_def
@@ -107,6 +42,10 @@ val _ = Portable.pprint Tag.pp_tag (tag symb_analysis_thm);
 
 Theorem chacha_other_line_symb_analysis_thm = symb_analysis_thm
 
+(* ------------------- *)
+(* first quarter round *)
+(* ------------------- *)
+
 val symb_analysis_thm =
  bir_symb_analysis_thm
   bir_chacha_prog_def
@@ -116,5 +55,19 @@ val symb_analysis_thm =
 val _ = Portable.pprint Tag.pp_tag (tag symb_analysis_thm);
 
 Theorem chacha_quarter_round_symb_analysis_thm = symb_analysis_thm
+
+(* ----------- *)
+(* first round *)
+(* ----------- *)
+
+val symb_analysis_thm =
+ bir_symb_analysis_thm
+  bir_chacha_prog_def
+  chacha_round_init_addr_def [chacha_round_end_addr_def]
+  bspec_chacha_round_pre_def chacha_birenvtyl_def;
+
+val _ = Portable.pprint Tag.pp_tag (tag symb_analysis_thm);
+
+Theorem chacha_round_symb_analysis_thm = symb_analysis_thm
 
 val _ = export_theory ();
